{
 "cells": [
  {
   "cell_type": "markdown",
   "metadata": {},
   "source": [
    "[![Open In Colab](https://colab.research.google.com/assets/colab-badge.svg)](https://colab.research.google.com/github/SeoulTechPSE/EngMath/blob/master/exams/final_2020_2_B.ipynb)"
   ]
  },
  {
   "cell_type": "markdown",
   "metadata": {},
   "source": [
    "## Engineering Mathematics II â€“ Final Exam."
   ]
  },
  {
   "cell_type": "markdown",
   "metadata": {},
   "source": [
    "**1.** $\\text{ }$ Find the eigenvalues and eigenfunctions of the problem:\n",
    "\n",
    "> $\\begin{align*}\n",
    "\\left [ (1 + x)^2 u' \\right ]' +\\lambda u &= 0,\\;\\; 0 < x < 1\\\\ \n",
    " u(0) = u(1) &= 0 \n",
    "\\end{align*}$\n",
    "\n",
    ">**HINT** $\\;\\;(1 +x)^{ia} = e^{ia \\ln (1 +x)}$\n",
    "\n",
    "**solution**\n",
    "\n",
    ">$\\begin{align*}\n",
    " &\\Downarrow 1 +x = t \\\\ \n",
    " t^2 \\frac{d^2 u}{dt^2} &+2t \\frac{du}{dt} +\\lambda u = 0, \\;\\;\\;\\text{Euler equation} \\\\ \n",
    " &\\Downarrow u = t^r \\\\ \n",
    " t^r &\\left[ r(r -1) +2r +\\lambda \\right] = 0\\\\ \n",
    " &\\Downarrow \\\\\n",
    " r &= -\\frac{1}{2} \\pm i \\frac{1}{2} \\sqrt{ 4\\lambda -1}, \\;\\; \\lambda > \\frac{1}{4} \\\\\n",
    " &\\Downarrow \\\\\n",
    " u(x) &= (1 +x)^{-\\frac{1}{2}} \\left[ c_1 \\cos \\left( \\frac{1}{2} \\sqrt{4\\lambda -1} \\ln(1 +x) \\right) \n",
    "      +c_2 \\sin \\left( \\frac{1}{2} \\sqrt{4\\lambda -1} \\ln(1 +x) \\right) \\right] \\\\\n",
    " &\\Downarrow  u(0) = u(1) = 0 \\\\ \n",
    " 0 &= c_1\\\\ \n",
    " 0 &= \\frac{1}{\\sqrt{2}} \\, c_2 \\, \\sin \\left(\\frac{\\ln2}{2} \\sqrt{4\\lambda -1} \\right ) \\;\\; \\Rightarrow \\;\\; \\frac{\\ln2}{2} \\sqrt{4\\lambda -1} = n\\pi, \\;\\;n=1,2,3,\\cdots \\\\\n",
    " &\\Downarrow \\\\\n",
    " \\text{Eigenvalues:}& \\;\\; \\lambda_n = \\left( \\frac{n\\pi}{\\ln2} \\right)^2 + \\frac{1}{4}, \\;\\; n= 1,2,3,\\cdots\\\\\n",
    " \\text{Eigenfunctions:}& \\;\\; u_n(x) = (1 +x)^{-\\frac{1}{2}} \\sin \\left[ \\frac{n\\pi}{\\ln2} \\ln(1 +x)\\right]\n",
    "\\end{align*}$"
   ]
  },
  {
   "cell_type": "markdown",
   "metadata": {},
   "source": [
    "**2.** $\\text{ }$ Solve\n",
    "\n",
    ">$\\begin{align*}\n",
    " u_t &= k \\,u_{xx}, \\;\\; a < x < b, \\;\\; t > 0 \\\\ \n",
    " &u(a, t) = 0 \\\\ \n",
    " &u(b, t) = 0 \\\\ \n",
    " &u(x, 0) = (x -a)(b -x)\n",
    "\\end{align*}$\n",
    "\n",
    "**solution** $\\text{ }$ \n",
    "\n",
    "> $\\begin{align*}\n",
    " &\\Downarrow \\;\\; \\hat{x} = x -a, \\;\\;\\hat{b}= b -a\\\\\n",
    " \\\\\n",
    " u_t &= k \\,u_{\\hat{x}\\hat{x}}, \\;\\; 0 < \\hat{x} < \\hat{b}, \\;\\; t > 0 \\\\ \n",
    " &u(0, t) = 0 \\\\ \n",
    " &u(\\hat{b}, t) = 0 \\\\ \n",
    " &u(\\hat{x}, 0) = \\hat{x}(\\hat{b} -x)\\\\\n",
    " \\\\\n",
    " &\\Downarrow u(\\hat{x}, t) = X(\\hat{x})T(t)\\\\\n",
    " \\\\\n",
    " u(\\hat{x}, t) &= \\sum_{n=1}^{\\infty}c_n \\exp \\left[ -k\\left( \\frac{n\\pi}{\\hat{b}}\\right)^2 t  \\right] \\sin \\frac{n\\pi\\hat{x}}{\\hat{b}} \\\\\n",
    " \\\\\n",
    " &\\Downarrow t=0\\\\\n",
    " \\\\\n",
    " \\hat{x}(\\hat{b} -\\hat{x}) &= \\sum_{n=1}^{\\infty}c_n \\sin \\frac{n\\pi\\hat{x}}{\\hat{b}} \\;\\;\\Rightarrow\\;\\;\n",
    " c_n = \\frac{2}{\\hat{b}} \\int_0^{\\hat{b}} \\,\\hat{x}(\\hat{b} -\\hat{x}) \\, \\sin \\frac{n\\pi\\hat{x}}{\\hat{b}}\\,d\\hat{x}\n",
    " =4\\frac{\\hat{b}^2}{(n\\pi)^3} \\left[ 1-(-1)^n \\right]\\\\\n",
    " \\\\\n",
    " &\\Downarrow\\\\\n",
    " \\\\\n",
    " u(x, t) &= \\frac{8(b -a)^2}{\\pi^3} \\sum_{n=1}^{\\infty}\\frac{1}{(2n -1)^3} \\exp \\left[ -k \\left( \\frac{(2n -1)\\pi}{b -a}\\right)^2 t  \\right] \\sin \\frac{(2n -1)\\pi(x-a)}{b -a}\n",
    " \\end{align*}$"
   ]
  },
  {
   "cell_type": "markdown",
   "metadata": {},
   "source": [
    "**3.** $\\text{ }$ Solve by separation of variables\n",
    "\n",
    ">$\\begin{align*}\n",
    " u_{tt} +u_t &= u_{xx},\\;\\;\\;0 < x < \\pi, \\;\\; t > 0 \\\\ \n",
    " u(0, t)&= 0\\\\ \n",
    " u_x(\\pi, t)&= 0\\\\ \n",
    " u(x, 0)&= \\sin^3 \\frac{x}{2}\\\\ \n",
    " u_t(x, 0)&= 0 \n",
    "\\end{align*}$\n",
    "\n",
    "**solution**\n",
    "\n",
    ">$\\begin{align*}\n",
    " &\\Downarrow \\;\\;  u(x,t) = X(x) T(t) \\\\\n",
    " \\\\\n",
    " \\frac{T'' +T'}{T} &= \\frac{X''}{X}=-\\lambda < 0 \\\\\n",
    " \\\\\n",
    " &\\Downarrow \\\\ \n",
    " \\\\\n",
    " X'' &+\\lambda X = 0, \\;\\;X(0)=X'(\\pi)=0 \\\\\n",
    " T'' &+T'+\\lambda T = 0 \\\\\n",
    " \\\\\n",
    " &\\Downarrow \\\\ \n",
    " \\\\\n",
    " \\lambda_n &= \\left( \\frac{2n-1}{2} \\right)^2, \\;\\;n=1,2,3,\\cdots \\\\\n",
    " X_n &= \\sin \\frac{2n-1}{2}x \\\\\n",
    " T_1 &= e^{-t/2} \\left( a_1 +b_1 t \\right) \\\\\n",
    " T_n &= e^{-t/2} \\left[ a_n \\cos \\left( \\sqrt{n(n -1)}\\, t\\right) +b_n \\sin \\left(\\sqrt{n(n -1)}\\, t\\right) \\right], \\;\\; n =2,3,\\cdots \\\\\n",
    " \\\\\n",
    " &\\Downarrow \\\\ \n",
    " \\\\\n",
    " u(x,t) &= e^{-t/2} \\left[ (a_1 +b_1 t) \\sin\\frac{x}{2} +\\sum_{n=2}^\\infty \\left(a_n \\cos \\sqrt{n(n-1)}\\, t +b_n \\sin \\sqrt{n(n-1)}\\, t \\right ) \\,\\sin \\frac{2n-1}{2}x\\right ] \\\\\n",
    " u_t(x,t) &= -\\frac{1}{2} u(x,t) \\;+\\; e^{-t/2} \\left[ b_1 \\sin\\frac{x}{2} +\\sum_{n=2}^\\infty \\left(-a_n \\sqrt{n(n-1)}\\sin \\sqrt{n(n-1)}\\, t +b_n \\sqrt{n(n-1)} \\cos \\sqrt{n(n-1)}\\, t \\right ) \\,\\sin \\frac{2n-1}{2}x\\right]\n",
    " \\\\ \\\\\n",
    " &\\Downarrow\\;\\;t=0 \\\\ \n",
    " \\\\\n",
    " u(x,0) &= \\sin^3\\frac{x}{2}=\\frac{3}{4} \\sin \\frac{1}{2}x -\\frac{1}{4} \\sin \\frac{3}{2}x = a_1 \\sin\\frac{1}{2}x +\\sum_{n=2}^\\infty a_n \\sin \\frac{2n -1}{2} x \\;\\;\\Rightarrow \\;\\; a_1 =\\frac{3}{4}, \\;\\;a_2 =-\\frac{1}{4} \\\\\n",
    " u_t(x,0) &= 0 =-\\frac{3}{8} \\sin\\frac{1}{2}x +\\frac{1}{8} \\sin \\frac{3}{2}x +b_1 \\sin\\frac{1}{2}x +\\sum_{n=2}^\\infty b_n \\sqrt{n(n-1)} \\sin\\frac{2n-1}{2}x \\;\\;\\Rightarrow \\;\\; b_1 =\\frac{3}{8}, \\;\\;b_2 =-\\frac{\\sqrt{2}}{16} \\\\\n",
    " \\\\\n",
    " &\\Downarrow \\\\ \n",
    " \\\\\n",
    " u(x,t) &= \\frac{1}{4} e^{-t/2} \\left[ 3\\left(1 +\\frac{1}{2}t\\right) \\sin \\frac{1}{2}x -\\left( \\cos \\sqrt{2}t +\\frac{\\sqrt{2}}{4} \\sin \\sqrt{2}t\\right) \\sin\\frac{3}{2}x  \\right]\n",
    "\\end{align*}$"
   ]
  },
  {
   "cell_type": "markdown",
   "metadata": {
    "cell_style": "center"
   },
   "source": [
    "**4.** $\\text{ }$ Solve \n",
    "\n",
    ">$\\begin{align*}\n",
    " \\nabla^2 u &= 0, \\;\\;\\;\\;\\;\\;\\;\\;\\;\\; r < 1 \\\\ \n",
    " u_r &= g(\\phi, \\theta), \\;\\; r=1 \n",
    "\\end{align*}$\n",
    "\n",
    "where\n",
    "\n",
    ">$\\displaystyle\\int_0^{2\\pi} \\int_0^\\pi g(\\phi,\\theta) \\, \\sin\\phi \\,d\\phi \\,d\\theta = 0$\n",
    "\n",
    "Let $u = 0$ at $r = 0$. What happens if this integral is not zero?  \n",
    "\n",
    "\n",
    "**solution**\n",
    "\n",
    "\n",
    ">$\\begin{align*}\n",
    "    \\nabla^2 u &=u_{rr} +\\frac{2}{r} u_r +\\frac{1}{r^2}u_{\\phi\\phi} +\\frac{\\cot\\phi}{r^2} u_{\\phi} +\\frac{1}{r^2\\sin^2\\phi}u_{\\theta\\theta} =0\\\\ \\\\\n",
    " &\\Downarrow \\;\\;  u(r,\\phi,\\theta) = R(r) \\Phi(\\phi) \\Theta(\\theta) \\\\\n",
    " \\\\\n",
    " - \\frac{r^2R''+2rR'}{R} \\sin^2 \\phi &- \\frac{\\left[ \\sin\\phi\\, \\Phi'\\right ]'}{\\Phi} \\sin\\phi=\\frac{\\Theta''}{\\Theta} = -\\mu < 0\\\\\n",
    " - \\frac{r^2R''+2rR'}{R} &= \\frac{\\left[ \\sin\\phi\\, \\Phi'\\right ]'}{\\sin\\phi\\,\\Phi} -\\frac{\\mu}{\\sin^2\\phi} = -\\lambda < 0 \\\\\n",
    " \\\\ \\Downarrow \\;\\;t=\\cos\\phi\\\\ \\\\\n",
    " \\Theta'' +\\mu \\Theta = 0,& \\;\\; \\Theta(0)=\\Theta(2\\pi), \\;\\;\\Theta'(0)=\\Theta'(2\\pi) \\;\\;\\Rightarrow \\;\\; \\mu_m = m^2, \\;\\;m=0,1,2,\\cdots, \\;\\;\\Theta_m(\\theta) =\\cos m\\theta, \\;\\sin m\\theta \\\\\n",
    " \\frac{d}{dt} \\left[ (1 -t^2) \\frac{d\\Phi}{dt}\\right] &- \\frac{m^2}{1-t^2} \\Phi +\\lambda \\Phi = 0, \\;\\;\\lambda_n =n(n+1), \\;\\;n=0,1,2,\\cdots,\\;\\;\\Phi_{mn}(t)=P_n^m(t) = (1 -t^2)^{m/2} \\frac{d^m}{dt^m}P_n(t)\\\\\n",
    " r^2 R_n'' +2r R_n'&-n(n+1)R_n = 0, \\;\\; R_n = r^n\\; (\\because u \\text{ is bounded}) \\\\ \\\\\n",
    " \\Downarrow \\\\\n",
    " u(r,\\phi,\\theta) = \\frac{1}{2} a_{00} &+\\sum_{n=1}^\\infty r^n \\left[ \\frac{1}{2}a_{n0} P_n(\\cos\\phi) +\\sum_{m=1}^n \n",
    "  \\left( a_{nm} \\cos m\\theta +b_{nm} \\sin m\\theta \\right) P_n^m(\\cos\\phi)\\right] \\\\ \\\\\n",
    "   &\\Downarrow \\;\\;u=0 \\;\\text{ at }\\; r=0\\;\\Rightarrow\\; a_{00}=0, \\;\\;u_r(1,\\phi,\\theta)=g(\\phi,\\theta)\\\\ \\\\\n",
    "   u_r(1,\\phi,\\theta) &= g(\\phi,\\theta)=\\sum_{n=1}^\\infty n \\left[ \\frac{1}{2}a_{n0} P_n(\\cos\\phi) +\\sum_{m=1}^n \n",
    "  \\left( a_{nm} \\cos m\\theta +b_{nm} \\sin m\\theta \\right) P_n^m(\\cos\\phi)\\right] \\\\\n",
    "  a_{nm}&=\\frac{1}{n\\pi}\\frac{(2n +1)}{2}\\frac{(n -m)!}{(n+m)!} \\,\\int_0^{2\\pi} \\int_0^\\pi g(\\phi,\\theta) \\cos m\\theta  \\,P_n^m(\\cos\\phi)\\,\\sin\\phi \\,d\\phi \\,d\\theta \\\\\n",
    "  b_{nm}&=\\frac{1}{n\\pi}\\frac{(2n +1)}{2}\\frac{(n -m)!}{(n+m)!} \\,\\int_0^{2\\pi} \\int_0^\\pi g(\\phi,\\theta) \\sin m\\theta  \\,P_n^m(\\cos\\phi)\\,\\sin\\phi \\,d\\phi \\,d\\theta \\\\\n",
    "\\end{align*}$\n",
    "\n",
    "> By the divergence theorem\n",
    "\n",
    "> $\\;\\;\\;\\displaystyle\\int_0^{2\\pi} \\int_0^\\pi \\int_0^1 (\\nabla^2 u) \\,r^2\\sin \\phi \\,dr\\,d\\phi\\,d\\theta = \\int_0^{2\\pi} \\int_0^\\pi \\frac{\\partial u}{\\partial r}(1,\\phi,\\theta) \\,\\sin\\phi \\,d\\phi\\,d\\theta$\n",
    "\n",
    "> Therefore if the integral on the right is not zero, $u$ cannot satisfy Laplace equation"
   ]
  }
 ],
 "metadata": {
  "kernelspec": {
   "display_name": "Python 3 (ipykernel)",
   "language": "python",
   "name": "python3"
  },
  "language_info": {
   "codemirror_mode": {
    "name": "ipython",
    "version": 3
   },
   "file_extension": ".py",
   "mimetype": "text/x-python",
   "name": "python",
   "nbconvert_exporter": "python",
   "pygments_lexer": "ipython3",
   "version": "3.9.18"
  }
 },
 "nbformat": 4,
 "nbformat_minor": 4
}
