{
 "cells": [
  {
   "cell_type": "markdown",
   "id": "a26af8d5",
   "metadata": {},
   "source": [
    "## Engineering Mathematics I (161006-21001) - Mid. Exam.\n",
    "April 11, 2022"
   ]
  },
  {
   "cell_type": "markdown",
   "id": "f492a544",
   "metadata": {},
   "source": [
    "**1[10].** $~$Solve\n",
    "\n",
    "> $\\displaystyle \\frac{dy}{dx}=\\frac{xy+3x-y-3}{xy -2x +4y-8}$\n",
    "\n",
    "$~$**solution**\n",
    "\n",
    "$$\n",
    "\\begin{align*}\n",
    "\\frac{dy}{dx} &= \\frac{(y+3)(x-1)}{(y-2)(x+4)} \\\\ \n",
    " &\\Downarrow \\\\ \n",
    " \\left ( 1-\\frac{5}{y+3} \\right )\\,dy &= \\left ( 1-\\frac{5}{x+4} \\right )\\, dx\\\\\n",
    " \\\\ \n",
    " y -5\\ln \\left| y+3 \\right| &= x -5\\ln \\left| x+4 \\right| +C\\\\\n",
    " \\\\ \n",
    " x -y + 5 \\ln &\\left| \\frac{y+3}{x+4}\\right| = C \n",
    "\\end{align*}\n",
    "$$\n"
   ]
  },
  {
   "cell_type": "markdown",
   "id": "67560fc1",
   "metadata": {},
   "source": [
    "**2[10].** $~$ Solve the given initial-value problem\n",
    "\n",
    "> $\\displaystyle y\\frac{dx}{dy} -x =2y^2, \\;\\;y(1)=5$\n",
    "\n",
    "$~$\n",
    "**solution**\n",
    "\n",
    "\\begin{align*}\n",
    " \\frac{dx}{dy} -\\frac{1}{y}x &= 2y, \\;\\;x(5) = 1\\\\ \n",
    " &\\Downarrow \\;\\; \\times \\;\\;\\frac{1}{y}  \\\\ \n",
    " \\frac{d}{dy} \\left ( \\frac{x}{y}\\right ) &= 2 \\\\ \n",
    " \\\\ \n",
    " \\frac{x}{y}&= 2y+C\\\\ \n",
    " &\\Downarrow \\;\\;x(5) = 1 \\\\\n",
    " x = y \\left ( 2y - \\frac{49}{5} \\right )\n",
    "\\end{align*}"
   ]
  },
  {
   "cell_type": "markdown",
   "id": "717470bb",
   "metadata": {},
   "source": [
    "**3[10].** $~$ Solve $\\cos x dx + \\left( 1+\\frac{2}{y} \\right)\\sin x dy=0$\n",
    "\n",
    "$~$\n",
    "**solution**\n",
    "\n",
    "\\begin{align*}\n",
    " &\\Downarrow \\times \\;\\; y^2 e^y \\\\\n",
    " y^2e^y \\cos x \\,dx &+ y^2 e^y \\left ( 1 + \\frac{2}{y} \\right ) \\sin x \\, dy = 0 \\\\ \n",
    " &\\Downarrow \\\\ \n",
    " \\frac{\\partial f}{\\partial x} = y^2 e^y \\cos x &\\;\\;\\Rightarrow\\;\\; f = y^2e^y \\sin x +h(y) \\\\ \n",
    " \\frac{\\partial f}{\\partial y} = y^2 e^y \\left ( 1 + \\frac{2}{y} \\right ) \\sin x +\\frac{dh}{dy}\\;\\; &\\Rightarrow \\;\\;\\frac{dh}{dy} = 0\\\\\n",
    " &\\Downarrow \\\\\n",
    " f &=  y^2e^y \\sin x +C = 0\n",
    "\\end{align*}"
   ]
  },
  {
   "cell_type": "markdown",
   "id": "8d4ac247",
   "metadata": {},
   "source": [
    "**4[10].** $~$Solve $~\\displaystyle \\frac{dy}{dx} = \\frac{x}{y} + \\frac{y}{x} +1$\n",
    "\n",
    "$~$\n",
    "\n",
    "\\begin{align*}\n",
    " &\\Downarrow \\;\\;y=ux, \\;\\;\\frac{dy}{dx}=u+x\\frac{du}{dx} \\\\ \n",
    " u + x\\frac{du}{dx} &= \\frac{1}{u} + u + 1 \\\\ \n",
    " \\left ( 1 - \\frac{1}{1+u} \\right ) du &= \\frac{1}{x} dx\\\\ \n",
    " &\\Downarrow \\\\ \n",
    " u - \\ln |1 + u| &= \\ln |x| +C \\\\\n",
    " &\\Downarrow \\\\\n",
    " \\frac{y}{x} -\\ln |x &+ y| = C \n",
    "\\end{align*}"
   ]
  },
  {
   "cell_type": "markdown",
   "id": "f3cb2812",
   "metadata": {},
   "source": [
    "**5[15].** $~$Solve $~y'' - 2y' + y = 4x^2 - 3 +x^{-1} e^x$\n",
    "\n",
    "$~$\n",
    "**solution**\n",
    "\n",
    "$$\n",
    "\\begin{align*}\n",
    "  y_h'' -2y_h' +y_h &= 0, \\;\\;y_{h_1} = e^x, \\;y_{h_2}=xe^x \\\\ \\\\\n",
    "  y_{p_1}'' -2y_{p_1}' +y_{p_1} &= 4x^2-3\\\\ \n",
    "  &\\Downarrow\\, y_{p_1} = Ax^2 + Bx + C \\\\\n",
    " y_{p_1} &= 2x^2 +8x +9 \\\\ \\\\\n",
    " y_{p_2}'' -2y_{p_2}' +y_{p_2} &= x^{-1} e^x \\\\\n",
    " W &= \\begin{vmatrix}\n",
    "       e^x & xe^x\\\\ \n",
    "       e^x & (1+x)e^x\n",
    "      \\end{vmatrix} = e^{2x} \\\\\n",
    " W_1 &= \\begin{vmatrix}\n",
    "         0 & xe^x\\\\ \n",
    "         x^{-1}e^x & (1+x)e^x \\\\\n",
    "        \\end{vmatrix} = -e^{2x} \\\\\n",
    " W_2 &= \\begin{vmatrix}\n",
    "          e^x & 0 \\\\ \n",
    "          e^x & x^{-1}e^x \\\\\n",
    "        \\end{vmatrix} = x^{-1} e^{2x} \\\\\n",
    "u_1 = \\int \\frac{W_1}{W} \\,dx = -x, &\\;\\;u_2 = \\int \\frac{W_2}{W}\\,dx = \\ln x \\\\\n",
    "&\\Downarrow \\\\\n",
    "y_{p_2} &=-xe^x + xe^x \\ln x\n",
    "\\end{align*}$$\n",
    "\n",
    "Then\n",
    "\n",
    "$$\n",
    "y = c_1e^x + c_2 xe^x +2x^2 +8x +9 -xe^x + +xe^x \\ln x\n",
    "$$"
   ]
  },
  {
   "cell_type": "markdown",
   "id": "ad89515e",
   "metadata": {},
   "source": [
    "**6[15].** Solve $x^2y'' -4xy' + 6y = 2x^4 + x^2$\n",
    "\n",
    "$~$\n",
    "**solution**\n",
    "\n",
    "\\begin{align*}\n",
    "x^2 y_h'' -4xy_h' +6y_h &= 0, \\;\\;y_{h_1} = x^2, \\;y_{h_2}=x^3 \\\\ \\\\\n",
    " y_{p}'' -\\frac{4}{x}y_{p}' +\\frac{6}{x^2}y_{p} &= 2x^2 +1 \\\\\n",
    " W &= \\begin{vmatrix}\n",
    "       x^2 & x^3\\\\ \n",
    "       2x & 3x^2\n",
    "      \\end{vmatrix} = x^4 \\\\\n",
    " W_1 &= \\begin{vmatrix}\n",
    "          0 & x^3\\\\ \n",
    "          2x^2+1 & 3x^2 \\\\\n",
    "        \\end{vmatrix} = -2x^5 -x^3 \\\\\n",
    " W_2 &= \\begin{vmatrix}\n",
    "          x^2 & 0 \\\\ \n",
    "          2x & 2x^2+1 \\\\\n",
    "        \\end{vmatrix} = 2x^4+x^2 \\\\\n",
    "u_1 = \\int \\frac{W_1}{W} \\,dx = -x^2 -\\ln x, &\\;\\;u_2 = \\int \\frac{W_2}{W}\\,dx = 2x -\\frac{1}{x} \\\\\n",
    "&\\Downarrow \\\\\n",
    "y_{p} &= x^4 -x^2 -x^2 \\ln x\n",
    "\\end{align*}\n",
    "\n",
    "Then\n",
    "\n",
    "$$y = c_1x^2 +c_2 x^3 +x^4 -x^2 -x^2 \\ln x$$"
   ]
  },
  {
   "cell_type": "markdown",
   "id": "da779d82",
   "metadata": {},
   "source": [
    "**7[15].** $~$Solve\n",
    "\n",
    "> $\\begin{align*}\n",
    " x' + y' &= t\\\\ \n",
    " 4x + y' &= 0\n",
    "\\end{align*} ~\\text{ at }  x(0)=1, y(0)=2$\n",
    "\n",
    "$~$\n",
    "**solution**\n",
    "\n",
    "\\begin{align*}\n",
    " &\\Downarrow \\;\\; \\text{Laplace Transform} \\\\ \n",
    " sX + sY &= 3 + \\frac{1}{s^2}\\\\ \n",
    " 4X + sY &= 2\\\\ \n",
    " &\\Downarrow \\\\ \n",
    " X &= \\frac{s^2 +1}{s^2(s-4)} = -\\frac{1}{16}\\cdot\\frac{1}{s} -\\frac{1}{4}\\cdot\\frac{1}{s^2} +\\frac{17}{16}\\cdot\\frac{1}{s-4} \\\\\n",
    " Y &= \\frac{2s^3-12s^2 - 4}{s^3(s-4)}=\\frac{49}{16}\\cdot\\frac{1}{s} +\\frac{1}{4}\\cdot\\frac{1}{s^2} +\\frac{1}{s^3}-\\frac{17}{16}\\cdot\\frac{1}{s-4}\\\\\n",
    " &\\Downarrow \\\\\n",
    " x(t) &= -\\frac{1}{16} -\\frac{1}{4}t +\\frac{17}{16} e^{4t} \\\\\n",
    " y(t) &= \\frac{49}{16} +\\frac{1}{4}t +\\frac{1}{2}t^2 -\\frac{17}{16} e^{4t}\n",
    "\\end{align*}"
   ]
  },
  {
   "cell_type": "markdown",
   "id": "5c81d569",
   "metadata": {},
   "source": [
    "**8[15].** $~$ One definition of the gamma function $\\Gamma(\\alpha)$ is given by the improper integral\n",
    "\n",
    "  >$\\displaystyle \\Gamma(\\alpha) =\\int_0^\\infty t^{\\alpha-1} e^{-t}\\,dt, \\;\\;\\alpha > 0$\n",
    "\n",
    "  > Use this definition to show that $\\Gamma(\\alpha + 1)=\\alpha \\Gamma(\\alpha)$ and show that\n",
    "  \n",
    "  >$\\displaystyle \\mathcal{L} \\{ t^\\alpha \\} = \\frac{\\Gamma (\\alpha+1)}{s^{\\alpha+1}}, \\;\\; \\alpha>-1$\n",
    "  \n",
    "$~$\n",
    "**solution**\n",
    "\n",
    "\\begin{align*}\n",
    " \\Gamma(\\alpha+1) &= \\int_0^\\infty t^\\alpha e^{-t} \\,dt \\\\ \n",
    " &= \\left. -t^\\alpha e^{-t} \\right|_0^\\infty + \\alpha\\int_0^\\infty t^{\\alpha-1} e^{-t}\\,dt \\\\ \n",
    " &= \\alpha \\Gamma(\\alpha)\\\\ \\\\\n",
    " \\mathcal{L}[t^\\alpha] &= \\int_0^\\infty t^\\alpha e^{-st} \\,dt \\\\\n",
    " &\\Downarrow \\,st=t', \\;\\;dt=\\frac{1}{s}dt' \\\\\n",
    " &=\\int_0^\\infty \\left( \\frac{t'}{s} \\right )^\\alpha e^{-t'} \\,\\frac{1}{s} \\,dt' \\\\\n",
    " &= \\frac{\\Gamma (\\alpha+1)}{s^{\\alpha+1}} \n",
    "\\end{align*}  "
   ]
  }
 ],
 "metadata": {
  "kernelspec": {
   "display_name": "Python 3 (ipykernel)",
   "language": "python",
   "name": "python3"
  },
  "language_info": {
   "codemirror_mode": {
    "name": "ipython",
    "version": 3
   },
   "file_extension": ".py",
   "mimetype": "text/x-python",
   "name": "python",
   "nbconvert_exporter": "python",
   "pygments_lexer": "ipython3",
   "version": "3.8.12"
  }
 },
 "nbformat": 4,
 "nbformat_minor": 5
}
